proved reasoning principle for mrec and eutt

theories/RuttFacts.v
@@ -22,6 +22,259 @@ Definition extract {E1 E2 A B} (REAns : relationEAnsH E1 E2)
   fun a b => REAns A B e1 a e2 b.
   
 
+Section Rutt6.
+
+Context (D1 D2 E1 E2 : Type -> Type).
+Context (REvE : relationEH E1 E2).
+Context (REvAns : forall A B : Type, E1 A -> A -> E2 B -> B -> Prop ).
+
+Context (REvInv : relationEH D1 D2).
+Context (REvAnsInv : forall A B : Type, D1 A -> A -> D2 B -> B -> Prop).
+
+Inductive rutt6F (sim : forall (A B : Type), D1 A -> D2 B -> itree E1 A -> itree E2 B -> Prop) :
+   forall (A B : Type), D1 A -> D2 B -> itree' E1 A -> itree' E2 B -> Prop := 
+  (* shows how the post condition of the itrees is reliant on d1 and d2*)
+  | rutt6RetF (A B : Type) (d1 : D1 A) (d2 : D2 B) a b : 
+    REvAnsInv A B d1 a d2 b -> rutt6F sim A B d1 d2 (RetF a) (RetF b)
+  | rutt6TauF (A B : Type) (d1 : D1 A) (d2 : D2 B) t1 t2 :
+    sim A B d1 d2 t1 t2 -> rutt6F sim A B d1 d2 (TauF t1) (TauF t2)
+  | rutt6VisF (A B C D : Type) (d1 : D1 A) (d2 : D2 B) (e1 : E1 C) (e2 : E2 D) k1 k2 :
+    REvE C D e1 e2 ->
+    (forall c d, REvAns C D e1 c e2 d -> sim A B d1 d2 (k1 c) (k2 d) ) ->
+    rutt6F sim A B d1 d2 (VisF e1 k1) (VisF e2 k2)
+
+  | rutt5TauL (A B : Type) (d1 : D1 A) (d2 : D2 B) t1 ot2 : 
+    rutt6F sim A B d1 d2 (observe t1) ot2 ->
+    rutt6F sim A B d1 d2 (TauF t1) ot2
+  | rutt5TauR (A B : Type) (d1 : D1 A) (d2 : D2 B) ot1 t2 : 
+    rutt6F sim A B d1 d2 ot1 (observe t2) ->
+    rutt6F sim A B d1 d2 ot1 (TauF t2)
+.
+
+Hint Constructors rutt6F : itree.
+
+Definition rutt6_ sim A B d1 d2 t1 t2 := rutt6F sim A B d1 d2 (observe t1) (observe t2).
+
+Hint Unfold rutt6_ : itree.
+
+Lemma rutt6_monot : monotone6 rutt6_.
+Proof.
+  repeat intro. red in IN. red.
+  induction IN; eauto with itree.
+Qed.
+
+
+
+Definition rutt6 : forall (A B : Type), D1 A -> D2 B -> itree E1 A -> itree E2 B -> Prop := paco6 rutt6_ bot6.
+
+#[local] Hint Resolve rutt6_monot : paco.
+
+Lemma rutt6_to_rutt (A B : Type) (d1 : D1 A) (d2 : D2 B) :
+  forall (t1 : itree E1 A) (t2 : itree E2 B), 
+    rutt6 A B d1 d2 t1 t2 ->
+    rutt REvE REvAns (extract REvAnsInv d1 d2) t1 t2.
+Proof.
+  pcofix CIH. intros t1 t2 Ht12. punfold Ht12. red in Ht12. pstep. red.
+  hinduction Ht12 before r; intros; pclearbot; eauto with itree.
+  - constructor; auto.
+  - constructor. right. apply CIH; auto.
+  - constructor; auto. intros. apply H0 in H1. pclearbot. right.
+    apply CIH; auto.
+  - constructor. eauto.
+  - constructor; eauto.
+Qed.
+
+Lemma rutt_to_rutt6 (A B : Type) (d1 : D1 A) (d2 : D2 B) :
+  forall (t1 : itree E1 A) (t2 : itree E2 B), 
+    rutt REvE REvAns (extract REvAnsInv d1 d2) t1 t2 ->
+    rutt6 A B d1 d2 t1 t2.
+Proof.
+  pcofix CIH. intros t1 t2 Ht12. punfold Ht12. red in Ht12. pstep. red.
+  hinduction Ht12 before r; intros; pclearbot; eauto with itree.
+  constructor; auto. intros. apply H0 in H1. pclearbot. right. apply CIH; auto.
+Qed.
+
+End Rutt6.
+
+#[global] Hint Resolve rutt6_monot : paco.
+
+Ltac use_simpobs := repeat match goal with
+                           | H : RetF _ = observe ?t |- _ => apply simpobs in H 
+                           | H : TauF _ = observe ?t |- _ => apply simpobs in H
+                           | H : VisF _ _ = observe ?t |- _ => apply simpobs in H
+                           end.
+
+Instance grutt_cong_eqit_eq {E1 E2 R1 R2 r rg} {RR : R1 -> R2 -> Prop} {REv RAns} :
+
+  Proper (@eq_itree E1 R1 R1 eq ==> @eq_itree E2 R2 R2 eq  ==> flip impl)
+         (gpaco2 (rutt_ REv RAns RR) (euttge_trans_clo RR) r rg  ).
+Proof. eapply grutt_cong_eqit; intros; subst; auto. Qed.
+
+Instance grutt_cong_euttge_eq {E1 E2 R1 R2 r rg} {RR : R1 -> R2 -> Prop} {REv RAns} :
+
+  Proper (@euttge E1 R1 R1 eq ==> @euttge E2 R2 R2 eq  ==> flip impl)
+         (gpaco2 (rutt_ REv RAns RR) (euttge_trans_clo RR) r rg  ).
+Proof. eapply grutt_cong_euttge; intros; subst; auto. Qed.
+
+(*move this to rutt theory*)
+Lemma rutt_bind (E1 E2 : Type -> Type) (R1 R2 S1 S2 : Type) (REvE : relationEH E1 E2) (REvAns : relationEAnsH E1 E2) 
+  (RR : R1 -> R2 -> Prop) (RS : S1 -> S2 -> Prop) k1 k2 :
+  (forall r1 r2, RR r1 r2 -> rutt REvE REvAns RS (k1 r1) (k2 r2) ) ->
+  forall t1 t2, rutt REvE REvAns RR t1 t2 -> rutt REvE REvAns RS (bind t1 k1) (bind t2 k2).
+Proof.
+  intros Hk. ginit. gcofix CIH. intros. punfold H0. red in H0.
+  remember (observe t1) as x. remember (observe t2) as y.
+  hinduction H0 before r; intros; use_simpobs.
+  - rewrite Heqx, Heqy. setoid_rewrite bind_ret_l. gfinal. right.
+    eapply paco2_mon; [eapply Hk; eauto | intros; contradiction].
+  - rewrite Heqx, Heqy. setoid_rewrite bind_tau. gstep. constructor.
+    gfinal. pclearbot. left. apply CIH. auto.
+  - rewrite Heqx, Heqy. setoid_rewrite bind_vis. gstep. constructor. auto.
+    intros. apply H0 in H1. pclearbot. gfinal. left. eapply CIH. auto.
+  - rewrite Heqx. rewrite tau_euttge. eauto.
+  - rewrite Heqy. rewrite tau_euttge. eauto.
+Qed.
+
+
+Variant EvEq {E : Type -> Type} : forall (A B : Type), E A -> E B -> Prop :=
+  | eveq (A : Type) (e : E A) : EvEq A A e e.
+
+
+
+Variant EvEqAns {E : Type -> Type} : forall A B, E A -> A -> E B -> B -> Prop :=
+  | eveqans A (e : E A) (a : A) : EvEqAns A A e a e a.
+
+Lemma rutt_to_eutt (E : Type -> Type) R1 R2 RR : 
+  forall (t1 : itree E R1) (t2 : itree E R2),
+    rutt EvEq EvEqAns RR t1 t2 -> eutt RR t1 t2.
+Proof.
+  ginit. gcofix CIH. intros t1 t2 Ht12. punfold Ht12. red in Ht12.
+  remember (observe t1) as ot1. remember (observe t2) as ot2.
+  hinduction Ht12 before r; intros; use_simpobs.
+  - rewrite Heqot1, Heqot2. gstep. constructor. auto.
+  - rewrite Heqot1, Heqot2. gstep. constructor. gfinal. left. pclearbot. eauto.
+  - rewrite Heqot1, Heqot2. dependent destruction H. gstep. constructor. intros.
+    gfinal. left. apply CIH. assert (EvEqAns A A e v e v). constructor. apply H0 in H. pclearbot. auto.
+  - rewrite Heqot1, tau_euttge. auto.
+  - rewrite Heqot2, tau_euttge. auto.
+Qed. 
+
+(*this is working fine but very annoying finish it monday morning*)
+Lemma rutt_cong_eqit_eql: forall (E1 E2 : Type -> Type) (R1 R2 : Type)
+                            (RR : R1 -> R2 -> Prop)
+                            (REv : forall A B : Type, E1 A -> E2 B -> Prop)
+                            (RAns : forall A B : Type, E1 A -> A -> E2 B -> B -> Prop)
+                            (b1 b2 : bool) (t1 t2 : itree E1 R1) (t4 : itree E2 R2),
+    eqit eq b1 b2 t1 t2 ->
+    rutt REv RAns RR t2 t4 -> rutt REv RAns RR t1 t4.
+Proof.
+  intros E1 E2 R1 R2 RR REv RAns b1 b2. ginit. gcofix CIH. 
+  intros t1 t2 t4 Ht12 Ht24. punfold Ht24. red in Ht24.
+  punfold Ht12. red in Ht12. remember (observe t1) as x.
+  remember (observe t2) as y. remember (observe t4) as z.
+  hinduction Ht24 before r; intros; use_simpobs.
+  - remember (RetF r1) as or. hinduction Ht12 before r; intros; inv Heqor; use_simpobs; eauto.
+    + rewrite Heqz. rewrite Heqx. gstep. constructor. auto.
+    + rewrite Heqx. rewrite tau_euttge. eauto.
+  - assert (DEC: (exists m3, x = TauF m3) \/ (forall m3, x <> TauF m3)).
+     { destruct x; eauto; right; repeat intro; discriminate. }
+     destruct DEC as [ [m3 Hm3]  | Hx ].
+     + subst. symmetry in Hm3. use_simpobs. rewrite Hm3, Heqz. gstep. constructor.
+       gfinal. left. pclearbot. eapply CIH; eauto. apply eqit_inv_Tau. rewrite <- Hm3.
+       pstep. auto.
+     + destruct x; try (exfalso; eapply Hx; eauto; fail).
+       {
+         pclearbot. use_simpobs. rewrite Heqx. clear Heqx t1. rewrite Heqz, tau_euttge. clear Heqz t4 Hx.
+         inv Ht12. punfold H. red in H. remember (RetF r0) as x.
+         hinduction REL before r; intros; inv Heqx; use_simpobs.
+         - gfinal. right. eapply paco2_mon; [ pstep; apply H | intros; contradiction].
+         - eapply IHREL; eauto. pstep_reverse. apply rutt_inv_Tau_l. pstep. auto.
+       }
+       {
+         pclearbot. rewrite Heqz, tau_euttge. use_simpobs. rewrite Heqx. inv Ht12. 
+         punfold H. red in H. remember (VisF e k) as x. hinduction REL before r; intros; inv Heqx0; inj_existT; subst.
+         - pclearbot. remember (VisF e0 k2) as x. remember (observe m2) as om2.
+           hinduction H before r; intros; inv Heqx0; inj_existT; subst.
+           + use_simpobs. rewrite Heqom2. gstep. constructor; auto. intros. apply H0 in H1.
+             pclearbot. gfinal. left. eapply CIH; eauto. apply REL.
+           + use_simpobs. rewrite Heqom2. rewrite tau_euttge. eauto.
+         - eapply IHREL; eauto. pstep_reverse. apply rutt_inv_Tau_l. pstep. auto.
+       }
+  - rewrite Heqz. remember (VisF e1 k1) as y. hinduction Ht12 before r; intros; inv Heqy0; inj_existT; subst; use_simpobs.
+    + rewrite Heqx. gstep. constructor; auto. intros. pclearbot. gfinal. left. eapply CIH; eauto.
+      apply REL. apply H0 in H1. pclearbot. auto.
+    + rewrite Heqx, tau_euttge; eauto.
+  - subst.
+    inv Ht12. pclearbot; use_simpobs.
+    + rewrite H0, tau_euttge. eapply IHHt24; eauto. pstep_reverse.
+    + use_simpobs. rewrite H0, tau_euttge. inv CHECK. eapply IHHt24; eauto. 
+      pstep_reverse. apply eqit_inv_Tau_r. pstep. auto.
+    + eapply IHHt24; eauto.
+  - rewrite Heqz, tau_euttge. eauto.
+Qed.
+
+Lemma rutt_cong_eqit_eqr: forall (E1 E2 : Type -> Type) (R1 R2 : Type)
+                            (RR : R1 -> R2 -> Prop)
+                            (REv : forall A B : Type, E1 A -> E2 B -> Prop)
+                            (RAns : forall A B : Type, E1 A -> A -> E2 B -> B -> Prop)
+                            (b1 b2 : bool) (t1 : itree E1 R1) (t2 t4 : itree E2 R2),
+    eqit eq b1 b2 t2 t4 ->
+    rutt REv RAns RR t1 t2 -> rutt REv RAns RR t1 t4.
+Proof.
+  intros E1 E2 R1 R2 RR REv RAns b1 b2. ginit. gcofix CIH. 
+  intros t1 t2 t4 Ht12 Ht24. punfold Ht24. red in Ht24.
+  punfold Ht12. red in Ht12. remember (observe t1) as x.
+  remember (observe t2) as y. remember (observe t4) as z.
+  hinduction Ht24 before r; intros; use_simpobs.
+  - remember (RetF r2) as or. hinduction Ht12 before r; intros; inv Heqor; use_simpobs; eauto.
+    + rewrite Heqz. rewrite Heqx. gstep. constructor. auto.
+    + rewrite Heqz. rewrite tau_euttge. eauto.
+  - assert (DEC: (exists m3, z = TauF m3) \/ (forall m3, z <> TauF m3)).
+     { destruct z; eauto; right; repeat intro; discriminate. }
+     destruct DEC as [ [m3 Hm3]  | Hz ].
+     + subst. symmetry in Hm3. use_simpobs. rewrite Hm3, Heqx. gstep. constructor.
+       gfinal. left. pclearbot. eapply CIH; eauto. apply eqit_inv_Tau. rewrite <- Hm3.
+       pstep. auto.
+     + destruct z; try (exfalso; eapply Hz; eauto; fail).
+       {
+         pclearbot. use_simpobs. rewrite Heqx. clear Heqx t1. rewrite Heqz, tau_euttge.
+         inv Ht12. punfold H. red in H. remember (RetF r0) as x.
+         hinduction REL before r; intros; inv Heqx; use_simpobs.
+         - gfinal. right. eapply paco2_mon; [ pstep; apply H | intros; contradiction].
+         - eapply IHREL; eauto. pstep_reverse. apply rutt_inv_Tau_r. pstep. auto.
+       }
+       {
+         pclearbot. use_simpobs. rewrite Heqz, Heqx, tau_euttge. inv Ht12. 
+         punfold H. red in H. remember (VisF e k) as x. hinduction REL before r; intros; inv Heqx0; inj_existT; subst.
+         - pclearbot. remember (VisF e0 k1) as x. remember (observe m1) as om2.
+           hinduction H before r; intros; inv Heqx0; inj_existT; subst.
+           + use_simpobs. rewrite Heqom2. gstep. constructor; auto. intros. apply H0 in H1.
+             pclearbot. gfinal. left. eapply CIH; eauto. apply REL.
+           + use_simpobs. rewrite Heqom2. rewrite tau_euttge. eauto.
+         - eapply IHREL; eauto. pstep_reverse. apply rutt_inv_Tau_r. pstep. auto.
+       }
+  - rewrite Heqx. remember (VisF e2 k2) as y. hinduction Ht12 before r; intros; inv Heqy0; inj_existT; subst; use_simpobs.
+    + rewrite Heqz. gstep. constructor; auto. intros. pclearbot. gfinal. left. eapply CIH; eauto.
+      apply REL. apply H0 in H1. pclearbot. auto.
+    + rewrite Heqz, tau_euttge; eauto.
+  - rewrite Heqx, tau_euttge. eapply IHHt24; eauto.
+  - inv Ht12. pclearbot; use_simpobs.
+    + rewrite H1, tau_euttge. eapply IHHt24; eauto. pstep_reverse.
+    + eapply IHHt24; eauto.
+    + use_simpobs. rewrite H0, tau_euttge. eapply IHHt24; eauto. inv CHECK. pstep_reverse.
+      eapply eqit_inv_Tau_l. pstep. auto.
+Qed.
+
+Instance rutt_cong_eqit_eq {E1 E2 R1 R2} {RR : R1 -> R2 -> Prop} {REv RAns} b1 b2 :
+  Proper (@eqit E1 R1 R1 eq b1 b2 ==> @eqit E2 R2 R2 eq b1 b2 ==> flip impl) (rutt REv RAns RR).
+Proof.
+  intros t1 t2 Ht12 t3 t4 Ht34 H.
+  eapply rutt_cong_eqit_eql; eauto. eapply rutt_cong_eqit_eqr; eauto. apply eqit_flip in Ht34. 
+  eapply eqit_mon; try apply Ht34; eauto.
+Qed.
+
+      
+
 Section MRec.
 
 Context (D1 D2 E : Type -> Type).
@@ -43,39 +296,153 @@ Context (Hbodies : forall A B (d1 : D1 A) (d2 : D2 B), REvInv A B d1 d2 ->
             (bodies1 A d1) (bodies2 B d2) ).
 (*maybe rutt actually needs to be changed? the types seem a little too constrained here
   if rutt took in a family of relations indexed by types? then there might be more hope *)
-Lemma rutt_mrec : 
+
+
+
+Instance eq_itree_Proper {E1 E2 R1 R2} {R : itree E1 R1 -> itree E2 R2 -> Prop} :  Proper (@eq_itree E1 R1 R1 eq ==> @eq_itree E2 R2 R2 eq ==> flip impl) R.                                                           
+Admitted. (* needs an axiom to prove this, can be more specific later, possibly even do some gpaco stuff, but for now I just
+             want to see how it works out *)
+
+
+Lemma rutt_mrec_interp_mrec_aux:
+  forall (A : Type) (d1 : D1 A) (B : Type) 
+    (d2 : D2 B)
+    (r : forall x x0 : Type, D1 x -> D2 x0 -> itree E x -> itree E x0 -> Prop),
+    (forall (A0 : Type) (init1 : D1 A0) (B0 : Type)
+       (init2 : D2 B0),
+        REvInv A0 B0 init1 init2 ->
+        r A0 B0 init1 init2 (mrec bodies1 init1) (mrec bodies2 init2)) ->
+    (forall (m1 : itree (D1 +' E) A) (m2 : itree (D2 +' E) B),
+        paco2
+          (rutt_ (sum_relE REvInv REvE) (sum_relAns REvAnsInv REvAns)
+                 (extract REvAnsInv d1 d2)) bot2 m1 m2 ->
+        r A B d1 d2 (interp_mrec bodies1 m1) (interp_mrec bodies2 m2)) ->
+    forall (m1 : itree (D1 +' E) A) (m2 : itree (D2 +' E) B),
+      paco2
+        (rutt_ (sum_relE REvInv REvE) (sum_relAns REvAnsInv REvAns)
+               (extract REvAnsInv d1 d2)) bot2 m1 m2 ->
+      paco6 (rutt6_ D1 D2 E E REvE REvAns REvAnsInv) r A B d1 d2
+            (interp_mrec bodies1 m1) (interp_mrec bodies2 m2).
+Proof.
+  intros A d1 B d2 r. intros CIH1 CIH2 m1 m2 Hm.
+  punfold Hm. red in Hm. remember (observe m1) as x. remember (observe m2) as y.
+  hinduction Hm before r; intros; use_simpobs.
+  - rewrite Heqx, Heqy. setoid_rewrite unfold_iter. cbn. setoid_rewrite bind_ret_l.
+    pstep. constructor; auto.
+  - pclearbot. rewrite Heqx, Heqy. setoid_rewrite unfold_iter.
+    cbn. setoid_rewrite bind_ret_l. pstep. constructor. right.
+    eapply CIH2; eauto.
+  - rewrite Heqx, Heqy. inversion H; inj_existT; subst.
+    + setoid_rewrite unfold_iter. cbn.
+      setoid_rewrite bind_ret_l. pstep. constructor. right. eapply CIH2.
+      eapply rutt_bind; eauto.
+      intros. red in H1.
+      eapply sum_relEAns_inl in H1. apply H0 in H1. pclearbot. auto.
+    + setoid_rewrite unfold_iter. cbn.
+      setoid_rewrite bind_vis. setoid_rewrite bind_ret_l.
+      pstep. constructor; auto. intros. left. pstep. constructor.
+      right. eapply CIH2; eauto. 
+      assert (sum_relAns REvAnsInv REvAns A0 B0 (inr1 f1) c (inr1 f2) d). constructor. auto.
+      apply H0 in H2. pclearbot. auto.
+  - rewrite Heqx. setoid_rewrite unfold_iter at 1. cbn. setoid_rewrite bind_ret_l.
+    pstep. constructor. pstep_reverse.
+  - rewrite Heqy. setoid_rewrite unfold_iter at 2. cbn. setoid_rewrite bind_ret_l.
+    pstep. constructor. pstep_reverse.
+Qed.
+(* ok so now I feel like I have a strong enough coinductive hypothesis, I have proved this up to one 
+   reasonable axiom (that I might be able to remove eventually) and one theorem that I expect to be true *)
+Theorem rutt_mrec : 
   forall A B (init1 : D1 A) (init2 : D2 B), 
-    (*need some constraints on RAB the problem is that RAB seems to need to be reliant
-      on init1 and init2, the return relation of two related calls depends on the 
-      actual call*)
     REvInv A B init1 init2 -> rutt REvE REvAns (extract REvAnsInv init1 init2)
          (mrec bodies1 init1) (mrec bodies2 init2).
 Proof.
-  ginit. gcofix CIH.
-  (* maybe I need some kind of 6? argument functor
-     A -> B -> D1 A -> D2 B -> itree ? A -> itree ? B -> Prop 
+  intros. apply rutt6_to_rutt. generalize dependent B. generalize dependent A.
+  pcofix CIH. unfold mrec. intros A d1 B d2 Hd12.
+  specialize (Hbodies A B d1 d2 Hd12) as Hbodiesd.
+  punfold Hbodiesd. red in Hbodiesd. remember (observe (bodies1 A d1)) as x.
+  remember (observe (bodies2 B d2)) as y. hinduction Hbodiesd before r; intros; use_simpobs; pclearbot.
+  - rewrite Heqx, Heqy. unfold interp_mrec. setoid_rewrite unfold_iter. setoid_rewrite bind_ret_l. 
+    pstep. constructor. auto.
+  - rewrite Heqx, Heqy. 
+    unfold interp_mrec at 1. rewrite unfold_iter. cbn. rewrite bind_ret_l.
+    fold (interp_mrec bodies1 m1).
+    unfold interp_mrec at 2. rewrite unfold_iter. cbn. rewrite bind_ret_l.
+    fold (interp_mrec bodies2 m2). pstep. constructor. left. 
+    clear Heqx Heqy. generalize dependent m2. revert m1.
+    pcofix CIH'. eapply rutt_mrec_interp_mrec_aux; eauto.
+  - (* this may be set up wrong*)
+    assert (Vis e1 k1 ≅ bind (trigger e1) k1 ). setoid_rewrite bind_trigger. reflexivity.
+    assert (Vis e2 k2 ≅ bind (trigger e2) k2 ). setoid_rewrite bind_trigger. reflexivity.
+    rewrite Heqx, Heqy. rewrite H1, H2. setoid_rewrite interp_mrec_bind. inversion H; inj_existT; subst; pclearbot.
+    + (*interp_mrec_trigger   : interp_mrec ctx (ITree.trigger a) ≳ mrecursive ctx U a *)
+      unfold interp_mrec at 1. rewrite unfold_iter. cbn. setoid_rewrite bind_ret_l. rewrite bind_tau.
+      fold (interp_mrec bodies1  (ITree.bind (bodies1 A0 e0) (fun x : A0 => Ret x))).
+      setoid_rewrite <- interp_mrec_bind.
+      unfold interp_mrec at 2. rewrite unfold_iter. cbn. rewrite bind_ret_l. setoid_rewrite bind_ret_l.
+      fold (interp_mrec bodies2  (ITree.bind (bodies2 _ e3) (fun x => k2 x))). setoid_rewrite bind_ret_r.
+      pstep. constructor. left. 
+      assert (Hb12 : rutt (sum_relE REvInv REvE)
+               (sum_relAns REvAnsInv REvAns)
+               (extract REvAnsInv d1 d2) (ITree.bind (bodies1 A0 e0) k1) (ITree.bind (bodies2 B0 e3) k2)).
+      { 
+        eapply rutt_bind; eauto.
+        intros. red in H3. eapply sum_relEAns_inl in H3. apply H0 in H3.
+        pclearbot. auto.
+      }
+      remember (ITree.bind (bodies1 A0 e0) k1) as t1.
+      remember (ITree.bind (bodies2 B0 e3) k2) as t2. clear Heqt1 Heqt2.
+      generalize dependent t2. generalize dependent t1. pcofix CIH'.
+      eapply rutt_mrec_interp_mrec_aux; eauto.
+    + unfold interp_mrec at 1. rewrite unfold_iter. cbn. rewrite bind_vis. setoid_rewrite bind_ret_l. 
+      rewrite bind_vis. setoid_rewrite unfold_iter at 1. cbn. setoid_rewrite bind_ret_l.
+      setoid_rewrite bind_tau. setoid_rewrite bind_ret_l. 
+      unfold interp_mrec at 2. rewrite unfold_iter. cbn. rewrite bind_vis. setoid_rewrite bind_ret_l. 
+      rewrite bind_vis. setoid_rewrite unfold_iter at 2. cbn. setoid_rewrite bind_ret_l.
+      setoid_rewrite bind_tau. setoid_rewrite bind_ret_l. pstep. constructor; auto.
+      intros. left. pstep. constructor. left.
+      assert (Hcd : sum_relAns REvAnsInv REvAns _ _ (inr1 f1) c (inr1 f2) d). econstructor. auto.
+      apply H0 in Hcd. pclearbot. remember (k1 c) as kc. remember (k2 d) as kd.
+      clear Heqkc Heqkd. generalize dependent kd. revert kc. pcofix CIH.
+      eapply rutt_mrec_interp_mrec_aux; eauto.
+  - rewrite Heqx. 
+    unfold interp_mrec at 1. rewrite unfold_iter. cbn. rewrite bind_ret_l.
+    fold (interp_mrec bodies1 t1). pstep. constructor. pstep_reverse. 
+    assert (Htd2 : rutt (sum_relE REvInv REvE)
+               (sum_relAns REvAnsInv REvAns)
+               (extract REvAnsInv d1 d2) t1 (bodies2 B d2) ).
+    {
+      apply Hbodies in Hd12.
+      assert (bodies1 A d1 ≈ t1). rewrite Heqx, tau_eutt. reflexivity. rewrite <- H. auto.
+    }
+    remember (bodies2 B d2) as t2. clear Heqx Heqy Heqt2 IHHbodiesd Hbodiesd. generalize dependent t2. generalize dependent t1.
+    pcofix CIH. intros. eapply rutt_mrec_interp_mrec_aux; eauto.
+  - rewrite Heqy. 
+    unfold interp_mrec at 2. rewrite unfold_iter. cbn. rewrite bind_ret_l.
+    fold (interp_mrec bodies2 t2). pstep. constructor. pstep_reverse. 
+    assert (Htd2 : rutt (sum_relE REvInv REvE)
+               (sum_relAns REvAnsInv REvAns)
+               (extract REvAnsInv d1 d2) (bodies1 A d1) t2 ).
+    {
+      apply Hbodies in Hd12.
+      assert (bodies2 _ d2 ≈ t2). rewrite Heqy, tau_eutt. reflexivity. rewrite <- H. auto.
+    }
+    remember (bodies1 _ d1) as t1. clear Heqx Heqy Heqt1 IHHbodiesd Hbodiesd. generalize dependent t2. generalize dependent t1.
+    pcofix CIH. intros. eapply rutt_mrec_interp_mrec_aux; eauto.
+Qed.
 
-     where the itrees are the tree generated by the mutually recusive call 
-     (there should be more arguments in the closure but these are the ones 
-      that vary coinductively?)
-
-      2 things to make sure that would actually be useful
-      1. strong enough to prove mrec rutt (or maybe just eutt) results
-               (in fact double implication is what I think I would want)
-      2. lets me have a coinductive hypothesis
-   *)
-  (*this is not good, I need to bring this up with steve on Thursday*)
-
-  (*wtf is going on here
-    the extract expression fixes the init 
-    I need to further generalize it in some way, but I am not really sure how
-    is it even correct behavior or are gpaco and paco acting up
-    I think the problem is that the functor relies on init1 and init2
-    if I could remove that, then I should be fine
-    but that is easier said than done
-   *)
-  unfold mrec, interp_mrec. intros Hinit. unfold extract. cbn.
-  setoid_rewrite unfold_iter.
-Admitted.
 End MRec.
   
+
+
+Theorem eutt_mrec (E D1 D2 : Type -> Type) (REvInv : relationEH D1 D2)  (REvAnsInv : forall A B : Type, D1 A -> A -> D2 B -> B -> Prop)
+  (bodies1 : D1 ~> itree (D1 +' E) ) (bodies2 : D2 ~> itree (D2 +' E) ) :
+  ( forall A B (d1 : D1 A) (d2 : D2 B), REvInv A B d1 d2 -> 
+         rutt (sum_relE REvInv EvEq) (sum_relAns REvAnsInv EvEqAns) (extract REvAnsInv d1 d2)
+            (bodies1 A d1) (bodies2 B d2) ) ->
+  forall A B (init1 : D1 A) (init2 : D2 B) , 
+    REvInv A B init1 init2 -> eutt (extract REvAnsInv init1 init2)
+         (mrec bodies1 init1) (mrec bodies2 init2).
+Proof.
+  intros.
+  eapply rutt_to_eutt. eapply rutt_mrec; eauto.
+Qed.
